lib: add some definitions and rules from rt branch
During the work on verifying the MCS kernel, many definitions
and rules were added to lib. This commit collects all of these,
with style improvements and some proof improvements.
In particular, this adds several results to deal with while loops,
such as corres_whileLoop

Signed-off-by: Michael McInerney <michael.mcinerney@proofcraft.systems>

lib/HaskellLib_H.thy
@@ -14,13 +14,14 @@ imports
   Lib
   More_Numeral_Type
   Monads.NonDetMonadVCG
+  Monads.OptionMonad
 begin
 
 abbreviation (input) "flip \<equiv> swp"
 
 abbreviation(input) bind_drop :: "('a, 'c) nondet_monad \<Rightarrow> ('a, 'b) nondet_monad
                       \<Rightarrow> ('a, 'b) nondet_monad" (infixl ">>'_" 60)
-  where "bind_drop \<equiv> (\<lambda>x y. bind x (K_bind y))"
+  where "bind_drop \<equiv> (\<lambda>x y. NonDetMonad.bind x (K_bind y))"
 
 lemma bind_drop_test:
   "foldr bind_drop x (return ()) = sequence_x x"
@@ -520,5 +521,13 @@ syntax (input)
   "_listcompr" :: "'a \<Rightarrow> lc_qual \<Rightarrow> lc_quals \<Rightarrow> 'a list"  ("[_ | __")
 
 lemma "[(x,1) . x \<leftarrow> [0..10]] = [(x,1) | x \<leftarrow> [0..10]]" by (rule refl)
+
+definition ohaskell_fail :: "unit list \<Rightarrow> ('s, 'a) lookup" where
+  "ohaskell_fail = K ofail"
+
+definition ohaskell_assert :: "bool \<Rightarrow> unit list \<Rightarrow> ('s, unit) lookup" where
+  "ohaskell_assert P ls \<equiv> if P then oreturn () else ofail"
+
+lemmas omonad_defs = omonad_defs ohaskell_assert_def ohaskell_fail_def
 
 end
