lib/Monads/NonDetMonadVCG.thy
@@ -556,6 +556,17 @@ lemma hoare_case_option_wp:
   \<Longrightarrow> \<lbrace>case_option P P' v\<rbrace> f v \<lbrace>\<lambda>rv. case v of None \<Rightarrow> Q rv | Some x \<Rightarrow> Q' x rv\<rbrace>"
   by (cases v) auto
 
+(* Might be useful for forward reasoning, when P is known. *)
+lemma hoare_when_cases:
+  "(\<And>s. \<not>B \<Longrightarrow> P s \<Longrightarrow> Q s)
+    \<Longrightarrow> (B \<Longrightarrow> \<lbrace> P \<rbrace> f \<lbrace> \<lambda>r. Q \<rbrace>)
+    \<Longrightarrow> \<lbrace> P \<rbrace> when B f \<lbrace> \<lambda>r. Q \<rbrace>"
+  by (cases B; simp add: valid_def return_def)
+
+lemma bind_dummy_ret_val:
+  "do y \<leftarrow> a; b od = do a; b od"
+  by simp
+
 subsection "Reasoning directly about states"
 
 lemma in_throwError:
@@ -657,6 +668,12 @@ lemma gets_the_in_monad:
 lemma in_alternative:
   "(r,s') \<in> fst ((f \<sqinter> g) s) = ((r,s') \<in> fst (f s) \<or> (r,s') \<in> fst (g s))"
   by (simp add: alternative_def)
+
+lemma use_valid_inv:
+  assumes step: "(r, s') \<in> fst (f s)"
+  assumes pres: "\<And>N. \<lbrace>\<lambda>s. N (P s) \<and> E s\<rbrace> f \<lbrace>\<lambda>rv s. N (P s)\<rbrace>"
+  shows "E s \<Longrightarrow> P s = P s'"
+  using use_valid[where f=f, OF step pres[where N="\<lambda>p. p = P s"]] by simp
 
 lemmas in_monad = inl_whenE in_whenE in_liftE in_bind in_bindE_L
                   in_bindE_R in_returnOk in_throwError in_fail
@@ -1247,6 +1264,10 @@ lemma hoare_vcg_conj_lift:
    apply (rule hoare_pre_imp [OF _ x], simp)
   apply (rule hoare_pre_imp [OF _ y], simp)
   done
+
+\<comment> \<open>A variant which works nicely with subgoals that do not contain schematics\<close>
+lemmas hoare_vcg_conj_lift_pre_fix
+  = hoare_vcg_conj_lift[where P=R and P'=R for R, simplified]
 
 lemma hoare_vcg_conj_liftE1:
   "\<lbrakk> \<lbrace>P\<rbrace> f \<lbrace>Q\<rbrace>,-; \<lbrace>P'\<rbrace> f \<lbrace>Q'\<rbrace>,\<lbrace>E\<rbrace> \<rbrakk> \<Longrightarrow>
@@ -1986,6 +2007,32 @@ lemma hoare_vcg_set_pred_lift_mono:
   assumes mono: "\<And>A B. A \<subseteq> B \<Longrightarrow> P A \<Longrightarrow> P B"
   shows "m \<lbrace> \<lambda>s. P {x. f x s} \<rbrace>"
   by (fastforce simp: valid_def elim!: mono[rotated] dest: use_valid[OF _ f])
+
+text \<open>If a function contains an @{term assert}, or equivalent, then it might be
+      possible to strengthen the precondition of an already-proven hoare triple
+      @{text pos}, by additionally proving a side condition @{text neg}, that
+      violating some condition causes failure. The stronger hoare triple produced
+      by this theorem allows the precondition to assume that the condition is
+      satisfied.\<close>
+lemma hoare_strengthen_pre_via_assert_forward:
+  assumes pos: "\<lbrace> P \<rbrace> f \<lbrace> Q \<rbrace>"
+  assumes rel: "\<And>s. S s \<longrightarrow> P s \<or> N s"
+  assumes neg: "\<lbrace> N \<rbrace> f \<lbrace> \<bottom>\<bottom> \<rbrace>"
+  shows "\<lbrace> S \<rbrace> f \<lbrace> Q \<rbrace>"
+  apply (rule hoare_weaken_pre)
+   apply (rule hoare_strengthen_post)
+    apply (rule hoare_vcg_disj_lift[OF pos neg])
+   by (auto simp: rel)
+
+text \<open>Like @{thm hoare_strengthen_pre_via_assert_forward}, strengthen a precondition
+      by proving a side condition that the negation of that condition would cause
+      failure. This version is intended for backward reasoning. Apply it to a goal to
+      obtain a stronger precondition after proving the side condition.\<close>
+lemma hoare_strengthen_pre_via_assert_backward:
+  assumes neg: "\<lbrace> Not \<circ> E \<rbrace> f \<lbrace> \<bottom>\<bottom> \<rbrace>"
+  assumes pos: "\<lbrace> P and E \<rbrace> f \<lbrace> Q \<rbrace>"
+  shows "\<lbrace> P \<rbrace> f \<lbrace> Q \<rbrace>"
+  by (rule hoare_strengthen_pre_via_assert_forward[OF pos _ neg], simp)
 
 
 section "validNF Rules"
